isabelle-thys/Expressions.thy
@@ -14,6 +14,65 @@ lift_definition rel_expression :: "(variable_raw \<Rightarrow> variable_raw \<Ri
 lemma rel_expression_eq: "rel_expression (=) (=) = (=)"
   unfolding rel_expression.rep_eq rel_set_eq rel_mem2_eq rel_fun_eq prod.rel_eq Rep_expression_inject by rule
 
+lemma left_unique_rel_expression[transfer_rule]:
+  assumes "left_unique R" and "left_unique S" and "right_total R" and "type_preserving_var_rel R"
+  shows "left_unique (rel_expression R S)"
+proof -
+  have "e = f" if "rel_expression R S e g" and "rel_expression R S f g" for e f g
+  proof -
+    obtain vse E where e: "Rep_expression e = (vse,E)" by (atomize_elim, auto)
+    obtain vsf F where f: "Rep_expression f = (vsf,F)" by (atomize_elim, auto)
+    obtain vsg G where g: "Rep_expression g = (vsg,G)" by (atomize_elim, auto)
+    from that have "rel_prod (rel_set R) (rel_fun (rel_mem2 R) S) (vse,E) (vsg,G)"
+      unfolding rel_expression.rep_eq e g by simp
+    then have vseg: "rel_set R vse vsg" and EG: "(rel_fun (rel_mem2 R) S) E G" by auto
+
+    from that have "rel_prod (rel_set R) (rel_fun (rel_mem2 R) S) (vsf,F) (vsg,G)"
+      unfolding rel_expression.rep_eq f g by simp
+    then have vsfg: "rel_set R vsf vsg" and FG: "(rel_fun (rel_mem2 R) S) F G" by auto
+
+    from vseg vsfg have "vse = vsf"
+      using \<open>left_unique R\<close>
+      by (meson left_uniqueD left_unique_rel_set) 
+
+    have left_unique_fun: "left_unique (rel_fun (rel_mem2 R) S)"
+      apply (rule left_unique_fun)
+       apply (rule left_total_rel_mem2)
+      using assms by auto
+    from EG FG have "E = F"
+      using left_unique_fun
+      by (meson left_uniqueD)
+
+    from \<open>vse = vsf\<close> \<open>E = F\<close>
+    show "e = f"
+      using Rep_expression_inject e f by fastforce
+    qed
+  then show ?thesis
+    unfolding left_unique_def by simp
+qed
+
+lemma rel_expression_flip[simp]: "(rel_expression R S)^--1 = rel_expression R^--1 S^--1"
+  apply (rule ext)+ unfolding conversep_iff apply transfer
+  using rel_mem2_flip[unfolded conversep_iff]
+  apply (auto simp: rel_fun_def rel_set_def)
+  by (metis (full_types))+
+
+lemma right_unique_rel_expression[transfer_rule]:
+  assumes "right_unique R" and "right_unique S" and "left_total R" and "type_preserving_var_rel R"
+  shows "right_unique (rel_expression R S)"
+  apply (subst conversep_conversep[of R, symmetric])
+  apply (subst conversep_conversep[of S, symmetric])
+  apply (subst rel_expression_flip[symmetric])
+  apply (simp del: rel_expression_flip)
+  apply (rule left_unique_rel_expression)
+  using assms by auto
+
+lemma bi_unique_rel_expression[transfer_rule]:
+  assumes "bi_unique R" and "bi_unique S" and "bi_total R" and "type_preserving_var_rel R"
+  shows "bi_unique (rel_expression R S)"
+  using assms by (meson bi_total_alt_def bi_unique_alt_def left_unique_rel_expression right_unique_rel_expression)
+
+
 lift_definition expression :: "'a::universe variables \<Rightarrow> ('a\<Rightarrow>'b) \<Rightarrow> 'b expression" is
   "\<lambda>(vs::'a variables) (f::'a\<Rightarrow>'b). (set (raw_variables vs), (f o eval_variables vs) :: mem2\<Rightarrow>'b)"
   using eval_variables_footprint by fastforce
@@ -81,6 +140,8 @@ qed
 
 lemma map_expression'[simp]: "map_expression' f (\<lambda>z. expression Q (e z)) = expression Q (\<lambda>a. f (\<lambda>z. e z a))"
   apply transfer by auto
+
+
 
 lift_definition pair_expression :: "'a expression \<Rightarrow> 'b expression \<Rightarrow> ('a \<times> 'b) expression" is
   "\<lambda>(vs1,e1) (vs2,e2). (vs1 \<union> vs2, \<lambda>m. (e1 m, e2 m))"
@@ -173,6 +234,86 @@ lemma index_flip_expression_vars[simp]: "expression_vars (index_flip_expression 
 lemma index_flip_expression_twice[simp]: "index_flip_expression (index_flip_expression e) = e"
   apply transfer by (auto simp: image_iff)
 
+
+lemma index_flip_expression_index_expression:
+  "index_flip_expression (index_expression left x) = index_expression (\<not>left) x"
+  apply transfer apply auto
+  using image_iff by fastforce
+
+(* lemma expression_vars_index_flip_expression: "expression_vars (index_flip_expression e) = index_flip_var_raw ` expression_vars e"
+  by (simp add: expression_vars.rep_eq index_flip_expression.rep_eq split_beta) *)
+
+lemma expression_eval_index_flip_expression: "expression_eval (index_flip_expression e) = 
+  expression_eval e o index_flip_mem2"
+  unfolding o_def
+  by (simp add: expression_eval.rep_eq index_flip_expression.rep_eq split_beta)
+
+lemma index_flip_expression_pair_expression: "index_flip_expression (pair_expression e1 e2)
+  = pair_expression (index_flip_expression e1) (index_flip_expression e2)"
+  apply transfer by auto
+
+lemma index_flip_expression_map_expression': "index_flip_expression (map_expression' f ez)
+  = map_expression' f (index_flip_expression o ez)"
+proof (cases "\<forall>z. expression_vars (ez z) = expression_vars (ez undefined)")
+  case True
+  then have True': "expression_vars (index_flip_expression (ez z)) = expression_vars (index_flip_expression (ez undefined))" for z
+    apply transfer
+    apply simp
+    by (metis (mono_tags, lifting) fst_conv split_beta)
+
+  from True have "expression_vars (map_expression' f ez) = expression_vars (ez undefined)"
+    apply transfer by (simp add: fst_def)
+  hence "expression_vars (index_flip_expression (map_expression' f ez)) 
+       = index_flip_var_raw ` expression_vars (ez undefined)"
+    unfolding index_flip_expression_vars by simp
+  moreover from True' have "expression_vars (map_expression' f (index_flip_expression o ez)) 
+      = expression_vars (index_flip_expression (ez undefined))"
+    unfolding o_def apply transfer by (auto simp: fst_def)
+  moreover have "expression_vars (index_flip_expression (ez undefined))
+      = index_flip_var_raw ` expression_vars (ez undefined)"
+    unfolding index_flip_expression_vars by simp
+  ultimately have vars: "expression_vars (index_flip_expression (map_expression' f ez))
+                 = expression_vars (map_expression' f (index_flip_expression o ez))"
+    by simp
+
+  from True have "expression_eval (map_expression' f ez) = (\<lambda>m. f (\<lambda>z. expression_eval (ez z) m))"
+    apply transfer by (auto simp: fst_def snd_def)
+  hence "expression_eval (index_flip_expression (map_expression' f ez)) 
+       = (\<lambda>m. f (\<lambda>z. expression_eval (ez z) (index_flip_mem2 m)))"
+    unfolding expression_eval_index_flip_expression by (simp add: o_def)
+  moreover from True' have "expression_eval (map_expression' f (index_flip_expression o ez)) 
+      = (\<lambda>m. f (\<lambda>z. expression_eval (index_flip_expression (ez z)) m))"
+    unfolding o_def apply transfer by (auto simp: fst_def snd_def)
+  moreover have "expression_eval (ez z) (index_flip_mem2 m) = expression_eval (index_flip_expression (ez z)) m" for m z
+    apply transfer by (simp add: split_beta)
+  ultimately have eval: "expression_eval (index_flip_expression (map_expression' f ez))
+                 = expression_eval (map_expression' f (index_flip_expression o ez))"
+    by simp
+  
+  from vars eval show ?thesis
+    by (rule expression_eqI)
+next
+  case False
+  then have False': "\<not> (\<forall>z. expression_vars (index_flip_expression (ez z)) = expression_vars (index_flip_expression (ez undefined)))"
+    apply transfer
+    apply (simp add: case_prod_beta)
+    using index_flip_var_raw_inject by blast
+
+  have "map_expression' f ez = const_expression undefined"
+    apply (subst Rep_expression_inject[symmetric])
+    using False by (auto simp: map_expression'.rep_eq expression_vars.rep_eq case_prod_beta)
+  then have "index_flip_expression (map_expression' f ez) = const_expression undefined"
+    by simp
+  also from False' have "map_expression' f (index_flip_expression o ez) = const_expression undefined"
+    apply (subst Rep_expression_inject[symmetric])
+    using False by (auto simp: map_expression'.rep_eq expression_vars.rep_eq case_prod_beta)
+  finally show ?thesis by metis
+qed
+
+lemma index_flip_map_expression2': "index_flip_expression (map_expression2' f e1 e2) = 
+  map_expression2' f (index_flip_expression e1) (index_flip_expression o e2)"
+  unfolding map_expression2'_def by (simp add: index_flip_expression_pair_expression index_flip_expression_map_expression' o_def)
+
 section \<open>Substitutions\<close>
 
 (* TODO move *)
@@ -205,6 +346,8 @@ lemma substitute1_variable[simp]: "substitution1_variable (substitute1 x e) = Re
 lemma substitute1_function: "substitution1_function (substitute1 x e) m = embedding (expression_eval e m)"
   apply transfer by auto
 
+
+
 lift_definition index_flip_substitute1 :: "substitution1 \<Rightarrow> substitution1" 
   is "\<lambda>(v,vs,f). (index_flip_var_raw v, index_flip_var_raw ` vs, f o index_flip_mem2)"
   by auto
@@ -213,11 +356,23 @@ lemma index_flip_substitute1: "index_flip_substitute1 (substitute1 x e) =
   substitute1 (index_flip_var x) (index_flip_expression e)"
   apply transfer by auto
 
-(* definition rel_substitute1 :: "(variable_raw\<Rightarrow>variable_raw\<Rightarrow>bool) \<Rightarrow> ('a expression\<Rightarrow>'a expression\<Rightarrow>bool) \<Rightarrow> (substitution1\<Rightarrow>substitution1\<Rightarrow>bool)" where
-  "rel_substitute1 rel_v rel_e s1 s2 = 
-    (rel_v (substitution1_variable s1) (substitution1_variable s2)
-   \<and> rel_e (inv embedding o substitution1_function s1) (substitution1_function s2))"
- *)
+lemma substitution1_variable_index_flip: "substitution1_variable (index_flip_substitute1 s) = 
+  index_flip_var_raw (substitution1_variable s)"
+  apply transfer by auto
+
+lemma substitution1_function_index_flip: "substitution1_function (index_flip_substitute1 s) = 
+  substitution1_function s \<circ> index_flip_mem2"
+  apply (cases "Rep_substitution1 s")
+  by (simp add: substitution1_function.rep_eq index_flip_substitute1.rep_eq)
+
+lemma index_flip_var_raw_substitution1_footprint: "index_flip_var_raw ` substitution1_footprint s =
+  substitution1_footprint (index_flip_substitute1 s)"
+  apply (cases "Rep_substitution1 s")
+  by (simp add: substitution1_footprint.rep_eq index_flip_substitute1.rep_eq)
+
+lemma index_flip_substitute1_twice[simp]: "index_flip_substitute1 (index_flip_substitute1 s) = s"
+  apply transfer by (auto simp: image_iff)
+
 
 definition rel_substitute1x :: "(variable_raw\<Rightarrow>variable_raw\<Rightarrow>bool) \<Rightarrow> (variable_raw\<Rightarrow>variable_raw\<Rightarrow>bool) \<Rightarrow> (substitution1\<Rightarrow>substitution1\<Rightarrow>bool)"
   where "rel_substitute1x R S s1 s2 \<longleftrightarrow> R (substitution1_variable s1) (substitution1_variable s2) \<and>
@@ -225,6 +380,7 @@ definition rel_substitute1x :: "(variable_raw\<Rightarrow>variable_raw\<Rightarr
     (rel_fun (rel_mem2 S) (=)) (substitution1_function s1) (substitution1_function s2)"
 
 
+(* Remove? *)
 lift_definition rel_substitute1 :: 
   "(variable_raw\<Rightarrow>variable_raw\<Rightarrow>bool) \<Rightarrow> ('a::universe expression\<Rightarrow>'b::universe expression\<Rightarrow>bool) 
           \<Rightarrow> (substitution1\<Rightarrow>substitution1\<Rightarrow>bool)" is
@@ -283,6 +439,129 @@ proof (rename_tac rel_v rel_exp1 rel_exp2 prod1 prod2)
     by (simp add: case_prod_beta prod1 prod2)
 qed
 
+lemma rel_substitute1_flip[simp]: "(rel_substitute1 R S)^--1 = rel_substitute1 R^--1 S^--1"
+  apply (rule ext)+ unfolding conversep_iff apply transfer by auto
+
+lemma rel_substitute1x_flip[simp]: "(rel_substitute1x R S)^--1 = rel_substitute1x R^--1 S^--1"
+  apply (rule ext)+ unfolding rel_substitute1x_def by (auto simp: rel_fun_def simp flip: rel_mem2_flip)
+
+lemma left_unique_rel_substitute1x[transfer_rule]: 
+  assumes "left_unique R"
+  assumes "left_unique S"
+    and "right_total S"
+    and "type_preserving_var_rel S"
+  shows "left_unique (rel_substitute1x R S)"
+proof (unfold rel_substitute1x_def, rule left_uniqueI, auto)
+  fix x y z
+  assume "R (substitution1_variable x) (substitution1_variable z)"
+    and "R (substitution1_variable y) (substitution1_variable z)"
+  with \<open>left_unique R\<close> have "substitution1_variable x = substitution1_variable y"
+    by (rule left_uniqueD)
+  moreover
+  assume "rel_set R (substitution1_footprint x) (substitution1_footprint z)"
+    and "rel_set R (substitution1_footprint y) (substitution1_footprint z)"
+  with \<open>left_unique R\<close> have "substitution1_footprint x = substitution1_footprint y"
+    by (meson left_uniqueD left_unique_rel_set)
+  moreover
+  assume "rel_fun (rel_mem2 S) (=) (substitution1_function x) (substitution1_function z)"
+    and "rel_fun (rel_mem2 S) (=) (substitution1_function y) (substitution1_function z)"
+  with assms have "substitution1_function x = substitution1_function y"
+    by (meson left_total_rel_mem2 left_uniqueD left_unique_eq left_unique_fun)
+  ultimately
+  show "x = y"
+    using Rep_substitution1_components Rep_substitution1_inject by auto
+qed
+
+lemma left_unique_rel_substitute1[transfer_rule]: 
+  assumes "left_unique R"
+  assumes "left_unique S"
+  shows "left_unique (rel_substitute1 R S)"
+proof -
+  have "s1 = s2" if "rel_substitute1 R S s1 t" and "rel_substitute1 R S s2 t" for s1 s2 t
+  proof -
+    obtain xs1 vss1 es1 where s1: "Rep_substitution1 s1 = (xs1,vss1,es1)" by (meson prod_cases3)
+    then have "finite vss1" and foot1: "(\<forall>w\<in>vss1. Rep_mem2 m1 w = Rep_mem2 m2 w) \<longrightarrow> es1 m1 = es1 m2" for m1 m2
+      using Rep_substitution1[of s1] by auto
+    obtain xs2 vss2 es2 where s2: "Rep_substitution1 s2 = (xs2,vss2,es2)" by (meson prod_cases3)
+    then have "finite vss2" and foot2: "(\<forall>w\<in>vss2. Rep_mem2 m1 w = Rep_mem2 m2 w) \<longrightarrow> es2 m1 = es2 m2" for m1 m2
+      using Rep_substitution1[of s2] by auto
+    obtain xt vst et where t: "Rep_substitution1 t = (xt,vst,et)" by (meson prod_cases3)
+
+    from that have "rel_prod R
+     (\<lambda>(vss1, es1) (vst, et).
+         range es1 \<subseteq> range EMBEDDING('a) \<and>
+         range et \<subseteq> range EMBEDDING('b) \<and>
+         S (Abs_expression (vss1, inv EMBEDDING('a) \<circ> es1)) (Abs_expression (vst, inv EMBEDDING('b) \<circ> et)))
+     (xs1, vss1, es1) (xt, vst, et)"
+      unfolding rel_substitute1.rep_eq s1 t by simp
+    then have R1: "R xs1 xt" and range_es1: "range es1 \<subseteq> range EMBEDDING('a)" and "range et \<subseteq> range EMBEDDING('b)" 
+      and S1: "S (Abs_expression (vss1, inv EMBEDDING('a) \<circ> es1)) (Abs_expression (vst, inv EMBEDDING('b) \<circ> et))"
+      by auto
+
+    from that have "rel_prod R
+     (\<lambda>(vss2, es2) (vst, et).
+         range es2 \<subseteq> range EMBEDDING('a) \<and>
+         range et \<subseteq> range EMBEDDING('b) \<and>
+         S (Abs_expression (vss2, inv EMBEDDING('a) \<circ> es2)) (Abs_expression (vst, inv EMBEDDING('b) \<circ> et)))
+     (xs2, vss2, es2) (xt, vst, et)"
+      unfolding rel_substitute1.rep_eq s2 t by simp
+    then have R2: "R xs2 xt" and range_es2: "range es2 \<subseteq> range EMBEDDING('a)" and "range et \<subseteq> range EMBEDDING('b)" 
+      and S2: "S (Abs_expression (vss2, inv EMBEDDING('a) \<circ> es2)) (Abs_expression (vst, inv EMBEDDING('b) \<circ> et))"
+      by auto
+
+    from R1 R2 have "xs1 = xs2"
+      using \<open>left_unique R\<close>
+      by (meson left_uniqueD)
+
+    from S1 S2 have AbsS: "Abs_expression (vss1, inv EMBEDDING('a) \<circ> es1) = Abs_expression (vss2, inv EMBEDDING('a) \<circ> es2)"
+      using \<open>left_unique S\<close>
+      by (meson left_uniqueD)
+    have "(vss1, inv EMBEDDING('a) \<circ> es1) = (vss2, inv EMBEDDING('a) \<circ> es2)"
+      apply (rule Abs_expression_inject[THEN iffD1, OF _ _ AbsS])
+      using foot1 foot2 \<open>finite vss1\<close> \<open>finite vss2\<close> by force+
+    then have "vss1 = vss2" and inv: "inv EMBEDDING('a) o es1 = inv EMBEDDING('a) o es2" by auto
+    with range_es1 range_es2 have "es1 = es2"
+      by (smt fun.inj_map_strong inv_into_injective subsetCE) 
+
+    from \<open>xs1 = xs2\<close> and \<open>vss1 = vss2\<close> and \<open>es1 = es2\<close>
+    show "s1 = s2"
+      using Rep_substitution1_inject s1 s2 by fastforce
+    qed
+  then show ?thesis
+    unfolding left_unique_def by simp
+qed
+
+lemma right_unique_rel_substitute1[transfer_rule]:
+  assumes "right_unique R" and "right_unique S"
+  shows "right_unique (rel_substitute1 R S)"
+  apply (subst conversep_conversep[of R, symmetric])
+  apply (subst conversep_conversep[of S, symmetric])
+  apply (subst rel_substitute1_flip[symmetric])
+  apply (simp del: rel_substitute1_flip)
+  apply (rule left_unique_rel_substitute1)
+  using assms by auto
+
+lemma right_unique_rel_substitute1x[transfer_rule]:
+  assumes "right_unique R" and "right_unique S" and "left_total S" and "type_preserving_var_rel S"
+  shows "right_unique (rel_substitute1x R S)"
+  apply (subst conversep_conversep[of R, symmetric])
+  apply (subst conversep_conversep[of S, symmetric])
+  apply (subst rel_substitute1x_flip[symmetric])
+  apply (simp del: rel_substitute1x_flip)
+  apply (rule left_unique_rel_substitute1x)
+  using assms by auto
+
+lemma bi_unique_rel_substitute1[transfer_rule]:
+  assumes "bi_unique R" and "bi_unique S"
+  shows "bi_unique (rel_substitute1 R S)"
+  using assms by (meson bi_total_alt_def bi_unique_alt_def left_unique_rel_substitute1 right_unique_rel_substitute1)
+
+lemma bi_unique_rel_substitute1x[transfer_rule]:
+  assumes "bi_unique R" and "bi_unique S" and "bi_total S" and "type_preserving_var_rel S"
+  shows "bi_unique (rel_substitute1x R S)"
+  using assms by (meson bi_total_alt_def bi_unique_alt_def left_unique_rel_substitute1x right_unique_rel_substitute1x)
+
+
 lemma rel_substitute1_expression_eq: "rel_substitute1 R (rel_expression S T) s1 s2 = 
         (R (substitution1_variable s1) (substitution1_variable s2) \<and>
         rel_set S (substitution1_footprint s1) (substitution1_footprint s2) \<and>
@@ -294,6 +573,28 @@ lemma rel_substitute1_expression_eq: "rel_substitute1 R (rel_expression S T) s1 
   apply transfer by force
 
 
+lemma rel_substitution1x_function:
+  includes lifting_syntax
+  fixes R S
+  defines "subR == rel_substitute1x R S"
+  shows "(subR ===> rel_mem2 S ===> (=)) substitution1_function substitution1_function"
+  unfolding subR_def rel_substitute1x_def apply (rule rel_funI)+ unfolding rel_fun_def
+  apply transfer by auto
+
+lemma rel_substitution1_function:
+  includes lifting_syntax
+  fixes R
+  defines "subR == rel_substitute1 R (rel_expression R (=))"
+  shows "(subR ===> rel_mem2 R ===> (=)) substitution1_function substitution1_function"
+proof (rule rel_funI, rule rel_funI, rename_tac s1 s2 m1 m2)
+  fix s1 s2 m1 m2
+  assume s12: "subR s1 s2"
+  assume m12: "rel_mem2 R m1 m2"
+  show "substitution1_function s1 m1 = substitution1_function s2 m2"
+    using s12 m12 unfolding subR_def 
+    apply transfer unfolding rel_fun_def rel_set_def apply auto
+    by (metis UNIV_I image_subset_iff inv_into_injective)
+qed
 
 
 lift_definition subst_mem2 :: "substitution1 list \<Rightarrow> mem2 \<Rightarrow> mem2" is
@@ -317,27 +618,6 @@ proof (rename_tac \<sigma> m v)
   qed
 qed
 
-
-(* lemma
-  includes lifting_syntax
-  fixes R
-  defines "subR == rel_substitute1 R (rel_expression R (=))"
-  shows "(subR ===> rel_prod R (rel_prod (rel_set R) (rel_mem2 R ===> (=)))) Rep_substitution1 Rep_substitution1"
-  apply (rule rel_funI)
-  apply (simp add: subR_def rel_substitute1_expression_eq[abs_def] rel_fun_def Rep_substitution1_components rel_prod_conv)
-  by (meson inv_into_injective rangeI set_rev_mp)
- *)
-
-(* lemma rel_substitute1_Rep_substitution1:
-  includes lifting_syntax
-  fixes R S
-  defines "subR == rel_substitute1 R (rel_expression R S)"
-  defines "S' == BNF_Greatest_Fixpoint.image2p embedding embedding S"
-  shows "(subR ===> rel_prod R (rel_prod (rel_set R) (rel_mem2 R ===> S'))) Rep_substitution1 Rep_substitution1"
-  apply (rule rel_funI)
-  apply (simp add: S'_def subR_def rel_substitute1_expression_eq[abs_def] rel_fun_def Rep_substitution1_components rel_prod_conv BNF_Greatest_Fixpoint.image2p_def)
-  apply auto
-  by (meson contra_subsetD f_inv_into_f rangeI) *)
 
 lemma rel_substitute1_Rep_substitution1:
   includes lifting_syntax
@@ -407,6 +687,89 @@ definition subst_expression :: "substitution list \<Rightarrow> 'b expression \<
   "subst_expression \<sigma> e =  *)
 
 
+lemma rel_subst_mem2_x:
+  includes lifting_syntax
+  fixes R
+  assumes [transfer_rule]: "bi_unique R"
+  defines "subR == rel_substitute1x R R"
+  shows "(list_all2 subR ===> rel_mem2 R ===> rel_mem2 R) subst_mem2 subst_mem2"
+proof (rule rel_funI, rule rel_funI)
+  fix s1 s2 m1 m2
+  assume s12[unfolded subR_def, transfer_rule]: "list_all2 subR s1 s2"
+  assume m12[transfer_rule]: "rel_mem2 R m1 m2"
+  show "rel_mem2 R (subst_mem2 s1 m1) (subst_mem2 s2 m2)"
+    unfolding rel_mem2.rep_eq subst_mem2.rep_eq 
+  proof (rule rel_funI, rename_tac v1 v2) 
+    fix v1 v2
+    assume v12[transfer_rule]: "R v1 v2"
+    note rel_substitute1x_substitution1_variable[transfer_rule]
+    define find1 find2 
+      where "find1 = find (\<lambda>s. substitution1_variable s = v1) s1" 
+        and "find2 = find (\<lambda>s. substitution1_variable s = v2) s2"
+    have find12: "(rel_option subR) find1 find2" 
+      unfolding find1_def find2_def subR_def
+      by transfer_prover
+    show "(case find1 of None \<Rightarrow> Rep_mem2 m1 v1 | Some s \<Rightarrow> substitution1_function s m1) =
+          (case find2 of None \<Rightarrow> Rep_mem2 m2 v2 | Some s \<Rightarrow> substitution1_function s m2)"
+    proof (cases "find1")
+      case None
+      with find12 have None2: "find2 = None" by auto
+      show ?thesis
+        unfolding None None2 apply simp
+        by (metis (full_types) v12 m12 rel_fun_def rel_mem2.rep_eq)
+    next
+      case (Some s1')
+      with find12 obtain s2' where Some2: "find2 = Some s2'" and [transfer_rule]: "subR s1' s2'"
+        by (meson option_rel_Some1)
+      have [transfer_rule]: "(subR ===> rel_mem2 R ===> (=)) substitution1_function substitution1_function"
+         unfolding subR_def by (rule rel_substitution1x_function)
+      show ?thesis
+        unfolding Some Some2 apply simp by transfer_prover
+    qed
+  qed
+qed
+
+lemma rel_subst_mem2:
+  includes lifting_syntax
+  fixes R
+  assumes [transfer_rule]: "bi_unique R"
+  defines "subR == rel_substitute1 R (rel_expression R (=))"
+  shows "(list_all2 subR ===> rel_mem2 R ===> rel_mem2 R) subst_mem2 subst_mem2"
+proof (rule rel_funI, rule rel_funI)
+  fix s1 s2 m1 m2
+  assume s12[unfolded subR_def, transfer_rule]: "list_all2 subR s1 s2"
+  assume m12[transfer_rule]: "rel_mem2 R m1 m2"
+  show "rel_mem2 R (subst_mem2 s1 m1) (subst_mem2 s2 m2)"
+    unfolding rel_mem2.rep_eq subst_mem2.rep_eq 
+  proof (rule rel_funI, rename_tac v1 v2) 
+    fix v1 v2
+    assume v12[transfer_rule]: "R v1 v2"
+    note rel_substitute1_substitution1_variable[transfer_rule]
+    define find1 find2 where "find1 = find (\<lambda>s. substitution1_variable s = v1) s1" and "find2 = find (\<lambda>s. substitution1_variable s = v2) s2"
+    have find12: "(rel_option subR) find1 find2" 
+      unfolding find1_def find2_def subR_def
+      by transfer_prover
+    show "(case find1 of None \<Rightarrow> Rep_mem2 m1 v1 | Some s \<Rightarrow> substitution1_function s m1) =
+          (case find2 of None \<Rightarrow> Rep_mem2 m2 v2 | Some s \<Rightarrow> substitution1_function s m2)"
+    proof (cases "find1")
+      case None
+      with find12 have None2: "find2 = None" by auto
+      show ?thesis
+        unfolding None None2 apply simp
+        by (metis (full_types) v12 m12 rel_fun_def rel_mem2.rep_eq)
+    next
+      case (Some s1')
+      with find12 obtain s2' where Some2: "find2 = Some s2'" and [transfer_rule]: "subR s1' s2'"
+        by (meson option_rel_Some1)
+      have [transfer_rule]: "(subR ===> rel_mem2 R ===> (=)) substitution1_function substitution1_function"
+         unfolding subR_def by (rule rel_substitution1_function)
+      show ?thesis
+        unfolding Some Some2 apply simp by transfer_prover
+    qed
+  qed
+qed
+
+
 lemma finite_substitution1_footprint[simp]: "finite (substitution1_footprint \<sigma>)"
   apply transfer by auto
 
@@ -436,6 +799,163 @@ qed
 lemma subst_expression_footprint_union:
   "subst_expression_footprint \<sigma> (X \<union> Y) = subst_expression_footprint \<sigma> X \<union> subst_expression_footprint \<sigma> Y"
   unfolding subst_expression_footprint_def by blast
+
+lemma rel_set_subst_expression_footprint_x:
+  includes lifting_syntax
+  assumes "bi_unique R" and "bi_total R" and "type_preserving_var_rel R"
+  defines "subR == rel_substitute1x R R"
+  assumes "list_all2 subR s1 s2"
+  assumes "rel_set R vs1 vs2" 
+  shows "rel_set R (subst_expression_footprint s1 vs1) (subst_expression_footprint s2 vs2)"
+proof (rule rel_setI)
+
+  have goal: "\<exists>y\<in>subst_expression_footprint s2 vs2. R x y" if "x \<in> subst_expression_footprint s1 vs1" 
+    and [transfer_rule]: "list_all2 subR s1 s2"
+    and [transfer_rule]: "rel_set R vs1 vs2"
+    and [transfer_rule]: "bi_unique R"
+    and [transfer_rule]: "bi_total R"
+    and [transfer_rule]: "type_preserving_var_rel R"
+    and subR_def: "subR = rel_substitute1x R R"
+  for x s1 s2 vs1 vs2 R subR
+  proof -
+    have [transfer_rule]: "(subR ===> R) substitution1_variable substitution1_variable"
+      unfolding subR_def by (rule rel_substitute1x_substitution1_variable)
+    have [transfer_rule]: "(subR ===> rel_set R) substitution1_footprint substitution1_footprint"
+      unfolding subR_def by (rule rel_substitute1x_substitution1_footprint)
+    have [transfer_rule]: "bi_unique subR" 
+      unfolding subR_def
+      using \<open>bi_unique R\<close> apply (rule bi_unique_rel_substitute1x)
+      using that bi_unique_eq by auto
+    show ?thesis
+    proof (cases "x \<in> vs1 - substitution1_variable ` set s1")
+      case False
+      with that obtain sx vx where x_sx: "x \<in> substitution1_footprint sx" 
+        and Some1: "Some sx = find (\<lambda>s. substitution1_variable s = vx) s1" 
+        and sx_vs1: "substitution1_variable sx \<in> vs1"
+        unfolding subst_expression_footprint_def by auto
+      from Some1 obtain i where s1i: "s1!i = sx" and lens1: "i < length s1"
+        by (metis find_Some_iff) 
+      define sy where "sy = s2!i"
+      then have [transfer_rule]: "subR sx sy"
+        using s1i lens1 \<open>list_all2 subR s1 s2\<close> list_all2_conv_all_nth by blast
+      from Some1 have vx_def: "vx = substitution1_variable sx"
+        by (metis (mono_tags) find_Some_iff)
+      define vy where "vy = substitution1_variable sy"
+      have [transfer_rule]: "R vx vy" unfolding vy_def vx_def
+        by (meson \<open>(subR ===> R) substitution1_variable substitution1_variable\<close> \<open>subR sx sy\<close> rel_funD)
+      from sx_vs1 have "vx : vs1"
+        by (simp add: vx_def)
+      have Some2: "Some sy = find (\<lambda>s. substitution1_variable s = vy) s2"
+        apply (transfer fixing: sy vy s1) 
+        by (fact Some1)
+      have sy_vs2: "substitution1_variable sy \<in> vs2"
+        apply (transfer fixing: sy vs2)
+        by (fact sx_vs1)
+      have "rel_set R (substitution1_footprint sx) (substitution1_footprint sy)"
+        by (meson \<open>(subR ===> rel_set R) substitution1_footprint substitution1_footprint\<close> \<open>subR sx sy\<close> rel_funD)
+      with x_sx obtain y where Rxy: "R x y" and y_sy: "y \<in> substitution1_footprint sy"
+        by (meson rel_set_def)
+      from Some2 sy_vs2 y_sy have "y\<in>subst_expression_footprint s2 vs2"
+        unfolding subst_expression_footprint_def by auto
+      with Rxy show ?thesis by auto
+    next
+      case True
+      have "rel_set R (vs1 - substitution1_variable ` set s1) (vs2 - substitution1_variable ` set s2)"
+        by transfer_prover
+      with True obtain y where "y \<in> vs2 - substitution1_variable ` set s2" and Rxy: "R x y"
+        by (meson rel_set_def)
+      then have "y\<in>subst_expression_footprint s2 vs2"
+        unfolding subst_expression_footprint_def by auto
+      with Rxy show ?thesis by auto 
+    qed
+  qed
+  show "\<exists>y\<in>subst_expression_footprint s2 vs2. R x y" if "x \<in> subst_expression_footprint s1 vs1" for x
+    apply (rule goal) using assms that by simp_all
+  show "\<exists>x\<in>subst_expression_footprint s1 vs1. R x y" if "y \<in> subst_expression_footprint s2 vs2" for y
+    apply (subst conversep_iff[of R, symmetric])
+    apply (rule goal[where R="conversep R" and subR="conversep subR"]) 
+          apply (simp_all add: list.rel_flip)
+    using that assms by (simp_all add: subR_def)
+qed
+
+lemma rel_set_subst_expression_footprint:
+  includes lifting_syntax
+  assumes "bi_unique R" and "bi_total R" and "type_preserving_var_rel R"
+  defines "subR == rel_substitute1 R (rel_expression R (=))"
+  assumes "list_all2 subR s1 s2"
+  assumes "rel_set R vs1 vs2" 
+  shows "rel_set R (subst_expression_footprint s1 vs1) (subst_expression_footprint s2 vs2)"
+proof (rule rel_setI)
+
+  have goal: "\<exists>y\<in>subst_expression_footprint s2 vs2. R x y" if "x \<in> subst_expression_footprint s1 vs1" 
+    and [transfer_rule]: "list_all2 subR s1 s2"
+    and [transfer_rule]: "rel_set R vs1 vs2"
+    and [transfer_rule]: "bi_unique R"
+    and [transfer_rule]: "bi_total R"
+    and [transfer_rule]: "type_preserving_var_rel R"
+    and subR_def: "subR = rel_substitute1 R (rel_expression R (=))"
+  for x s1 s2 vs1 vs2 R subR
+  proof -
+    have [transfer_rule]: "(subR ===> R) substitution1_variable substitution1_variable"
+      unfolding subR_def by (rule rel_substitute1_substitution1_variable)
+    have [transfer_rule]: "(subR ===> rel_set R) substitution1_footprint substitution1_footprint"
+      unfolding subR_def by (rule rel_substitute1_substitution1_footprint)
+    have [transfer_rule]: "bi_unique subR" 
+      unfolding subR_def
+      using \<open>bi_unique R\<close> apply (rule bi_unique_rel_substitute1)
+      apply (rule bi_unique_rel_expression)
+      using that bi_unique_eq by auto
+    show ?thesis
+    proof (cases "x \<in> vs1 - substitution1_variable ` set s1")
+      case False
+      with that obtain sx vx where x_sx: "x \<in> substitution1_footprint sx" 
+        and Some1: "Some sx = find (\<lambda>s. substitution1_variable s = vx) s1" 
+        and sx_vs1: "substitution1_variable sx \<in> vs1"
+        unfolding subst_expression_footprint_def by auto
+      from Some1 obtain i where s1i: "s1!i = sx" and lens1: "i < length s1"
+        by (metis find_Some_iff) 
+      define sy where "sy = s2!i"
+      then have [transfer_rule]: "subR sx sy"
+        using s1i lens1 \<open>list_all2 subR s1 s2\<close> list_all2_conv_all_nth by blast
+      from Some1 have vx_def: "vx = substitution1_variable sx"
+        by (metis (mono_tags) find_Some_iff)
+      define vy where "vy = substitution1_variable sy"
+      have [transfer_rule]: "R vx vy" unfolding vy_def vx_def
+        by (meson \<open>(subR ===> R) substitution1_variable substitution1_variable\<close> \<open>subR sx sy\<close> rel_funD)
+      from sx_vs1 have "vx : vs1"
+        by (simp add: vx_def)
+      have Some2: "Some sy = find (\<lambda>s. substitution1_variable s = vy) s2"
+        apply (transfer fixing: sy vy s1) 
+        by (fact Some1)
+      have sy_vs2: "substitution1_variable sy \<in> vs2"
+        apply (transfer fixing: sy vs2)
+        by (fact sx_vs1)
+      have "rel_set R (substitution1_footprint sx) (substitution1_footprint sy)"
+        by (meson \<open>(subR ===> rel_set R) substitution1_footprint substitution1_footprint\<close> \<open>subR sx sy\<close> rel_funD)
+      with x_sx obtain y where Rxy: "R x y" and y_sy: "y \<in> substitution1_footprint sy"
+        by (meson rel_set_def)
+      from Some2 sy_vs2 y_sy have "y\<in>subst_expression_footprint s2 vs2"
+        unfolding subst_expression_footprint_def by auto
+      with Rxy show ?thesis by auto
+    next
+      case True
+      have "rel_set R (vs1 - substitution1_variable ` set s1) (vs2 - substitution1_variable ` set s2)"
+        by transfer_prover
+      with True obtain y where "y \<in> vs2 - substitution1_variable ` set s2" and Rxy: "R x y"
+        by (meson rel_set_def)
+      then have "y\<in>subst_expression_footprint s2 vs2"
+        unfolding subst_expression_footprint_def by auto
+      with Rxy show ?thesis by auto 
+    qed
+  qed
+  show "\<exists>y\<in>subst_expression_footprint s2 vs2. R x y" if "x \<in> subst_expression_footprint s1 vs1" for x
+    apply (rule goal) using assms that by simp_all
+  show "\<exists>x\<in>subst_expression_footprint s1 vs1. R x y" if "y \<in> subst_expression_footprint s2 vs2" for y
+    apply (subst conversep_iff[of R, symmetric])
+    apply (rule goal[where R="conversep R" and subR="conversep subR"]) 
+          apply (simp_all add: list.rel_flip)
+    using that assms by (simp_all add: subR_def)
+qed
 
 lemma subst_mem2_footprint:
   fixes \<sigma> vs
@@ -468,6 +988,7 @@ next
     by (simp add: Rep_sf)
 qed
 
+
 lift_definition subst_expression :: "substitution1 list \<Rightarrow> 'b expression \<Rightarrow> 'b expression" is
   "\<lambda>(\<sigma>::substitution1 list) (vs,e).
        (subst_expression_footprint \<sigma> vs,
@@ -489,6 +1010,105 @@ lemma subst_expression_footprint: "expression_vars (subst_expression \<sigma> e)
   apply transfer by auto
 lemma subst_expression_eval: "expression_eval (subst_expression \<sigma> e) = expression_eval e o subst_mem2 \<sigma>"
   apply (rule ext) unfolding o_def expression_eval.rep_eq subst_expression.rep_eq case_prod_beta by simp
+
+
+lemma rel_expression_subst_expression [transfer_rule]: 
+  includes lifting_syntax
+  assumes [transfer_rule]: "bi_unique R" and [transfer_rule]: "bi_total R" and [transfer_rule]: "type_preserving_var_rel R"
+  defines "subR == rel_substitute1 R (rel_expression R (=))"
+  shows "(list_all2 subR ===> rel_expression R (=) ===> rel_expression R (=)) 
+         subst_expression subst_expression"
+proof -
+  have "rel_expression R (=) (subst_expression s1 e1) (subst_expression s2 e2)" 
+    if subR_s1_s2[transfer_rule]: "list_all2 subR s1 s2" and R_e1_e2: "rel_expression R (=) e1 e2" 
+    for s1 s2 and e1 e2 :: "'b expression"
+  proof -
+    define vs1 E1 vs2 E2 where "vs1 = expression_vars e1" and "E1 = expression_eval e1"
+      and "vs2 = expression_vars e2" and "E2 = expression_eval e2"
+    have [unfolded subR_def, transfer_rule]: "(subR ===> rel_prod R (rel_prod (rel_set R) (rel_mem2 R ===> (=)))) Rep_substitution1 Rep_substitution1"
+      unfolding subR_def apply (rule rel_substitute1_Rep_substitution1) by simp
+    have [transfer_rule]: "(subR ===> R) substitution1_variable substitution1_variable"
+      unfolding subR_def by (rule rel_substitute1_substitution1_variable)
+    have [transfer_rule]: "bi_unique subR" 
+      unfolding subR_def
+      using \<open>bi_unique R\<close> apply (rule bi_unique_rel_substitute1)
+      apply (rule bi_unique_rel_expression)
+      using assms bi_unique_eq by auto
+    have [transfer_rule]: "(subR ===> rel_set R) substitution1_footprint substitution1_footprint"
+      unfolding subR_def by (rule rel_substitute1_substitution1_footprint)
+    have R_vs1_vs2[transfer_rule]: "rel_set R vs1 vs2"
+      unfolding vs1_def vs2_def using R_e1_e2 apply transfer by auto
+    have foot: "rel_set R (subst_expression_footprint s1 vs1) (subst_expression_footprint s2 vs2)"
+      apply (rule rel_set_subst_expression_footprint)
+      using assms R_vs1_vs2 subR_s1_s2 unfolding subR_def by auto
+    have E1E2: "(rel_mem2 R ===> (=)) E1 E2" 
+      unfolding E1_def E2_def apply (rule rel_funI)
+      using R_e1_e2 apply transfer 
+      unfolding rel_mem2.rep_eq rel_fun_def by auto
+    have subst_mem2_s1_s2: "(rel_mem2 R ===> rel_mem2 R) (subst_mem2 s1) (subst_mem2 s2)"
+      using rel_subst_mem2 subR_s1_s2 \<open>bi_unique R\<close>
+      by (metis rel_fun_def subR_def)
+    from E1E2 subst_mem2_s1_s2 have subst: "(rel_mem2 R ===> (=)) (E1 \<circ> subst_mem2 s1) (E2 \<circ> subst_mem2 s2)"
+      by (smt comp_def rel_funD rel_funI)
+    show ?thesis
+      unfolding rel_expression.rep_eq subst_expression.rep_eq using foot subst
+      by (simp add: Rep_expression_components E1_def E2_def vs1_def vs2_def)
+  qed
+
+  then show ?thesis
+     unfolding subR_def
+    apply (rule_tac rel_funI)+ by assumption
+qed
+
+lemma rel_expression_subst_expression_x [transfer_rule]: 
+  includes lifting_syntax
+  fixes R
+  assumes [transfer_rule]: "bi_unique R" and [transfer_rule]: "bi_total R" and [transfer_rule]: "type_preserving_var_rel R"
+  defines "subR == rel_substitute1x R R"
+  shows "(list_all2 subR ===> rel_expression R (=) ===> rel_expression R (=)) 
+         subst_expression subst_expression"
+proof -
+  have "rel_expression R (=) (subst_expression s1 e1) (subst_expression s2 e2)" 
+    if subR_s1_s2[transfer_rule]: "list_all2 subR s1 s2" and R_e1_e2: "rel_expression R (=) e1 e2" 
+    for s1 s2 and e1 e2 :: "'b expression"
+  proof -
+    define vs1 E1 vs2 E2 where "vs1 = expression_vars e1" and "E1 = expression_eval e1"
+      and "vs2 = expression_vars e2" and "E2 = expression_eval e2"
+    have [unfolded subR_def, transfer_rule]: 
+      "(subR ===> rel_prod R (rel_prod (rel_set R) (rel_mem2 R ===> (=)))) Rep_substitution1 Rep_substitution1"
+      unfolding subR_def by (rule rel_substitute1x_Rep_substitution1)
+    have [transfer_rule]: "(subR ===> R) substitution1_variable substitution1_variable"
+      unfolding subR_def by (rule rel_substitute1x_substitution1_variable)
+    have [transfer_rule]: "bi_unique subR" 
+      unfolding subR_def
+      using \<open>bi_unique R\<close> apply (rule bi_unique_rel_substitute1x)
+      by (auto simp: assms)
+    have [transfer_rule]: "(subR ===> rel_set R) substitution1_footprint substitution1_footprint"
+      unfolding subR_def by (rule rel_substitute1x_substitution1_footprint)
+    have R_vs1_vs2[transfer_rule]: "rel_set R vs1 vs2"
+      unfolding vs1_def vs2_def using R_e1_e2 apply transfer by auto
+    have foot: "rel_set R (subst_expression_footprint s1 vs1) (subst_expression_footprint s2 vs2)"
+      apply (rule rel_set_subst_expression_footprint_x)
+      using assms R_vs1_vs2 subR_s1_s2 unfolding subR_def by auto
+    have E1E2: "(rel_mem2 R ===> (=)) E1 E2" 
+      unfolding E1_def E2_def apply (rule rel_funI)
+      using R_e1_e2 apply transfer 
+      unfolding rel_mem2.rep_eq rel_fun_def by auto
+    have subst_mem2_s1_s2: "(rel_mem2 R ===> rel_mem2 R) (subst_mem2 s1) (subst_mem2 s2)"
+      using rel_subst_mem2_x subR_s1_s2 \<open>bi_unique R\<close>
+      by (metis rel_fun_def subR_def)
+    from E1E2 subst_mem2_s1_s2 have subst: "(rel_mem2 R ===> (=)) (E1 \<circ> subst_mem2 s1) (E2 \<circ> subst_mem2 s2)"
+      by (smt comp_def rel_funD rel_funI)
+    show ?thesis
+      unfolding rel_expression.rep_eq subst_expression.rep_eq using foot subst
+      by (simp add: Rep_expression_components E1_def E2_def vs1_def vs2_def)
+  qed
+
+  then show ?thesis
+     unfolding subR_def
+    apply (rule_tac rel_funI)+ by assumption
+qed
+
 
 lemma subst_expression_unit_tac:
   shows "expression variable_unit E = subst_expression s (expression variable_unit E)"
@@ -618,6 +1238,77 @@ proof (subst Rep_expression_inject[symmetric], simp add: expression.rep_eq subst
     by auto
 qed
 
+
+lemma index_flip_subst_expression: 
+  fixes \<sigma> :: "substitution1 list" and e :: "'a expression"
+  shows "index_flip_expression (subst_expression \<sigma> e) 
+        = subst_expression (map index_flip_substitute1 \<sigma>) (index_flip_expression e)"
+proof -
+  define subR where "subR = (rel_substitute1x rel_flip_index rel_flip_index)" 
+  
+  have rel_set_rel_flip_index: "rel_set rel_flip_index x y \<longleftrightarrow> index_flip_var_raw ` x = y" for x y
+    unfolding rel_set_def rel_flip_index_def by auto
+
+  include lifting_syntax
+  note bi_unique_rel_flip_index[transfer_rule]
+  note bi_total_rel_flip_index[transfer_rule]
+  note type_preserving_rel_flip_index[transfer_rule]
+
+  have rel_fun_flip[simp]: "(x ===> y)^--1 = (x^--1 ===> y^--1)" for x :: "'c\<Rightarrow>'d\<Rightarrow>bool" and y :: "'e\<Rightarrow>'f\<Rightarrow>bool" 
+    unfolding rel_fun_def by auto
+
+  have "rel_expression rel_flip_index (=) e (index_flip_expression e)" for e :: "'c expression"
+  proof (unfold rel_expression.rep_eq index_flip_expression.rep_eq, cases "Rep_expression e", auto)
+    fix vs f assume "Rep_expression e = (vs,f)"
+    show "rel_set rel_flip_index vs (index_flip_var_raw ` vs)"
+      by (rule rel_setI, unfold rel_flip_index_def, auto)
+    show "(rel_mem2 rel_flip_index ===> (=)) f (\<lambda>m. f (index_flip_mem2 m))"
+      apply (rule conversepD[of "(rel_mem2 rel_flip_index ===> (=))"])
+      unfolding rel_fun_flip apply simp
+      unfolding rel_fun_def rel_mem2.rep_eq rel_flip_index_def'
+      unfolding rel_flip_index_def' apply transfer by auto
+  qed
+  then have [transfer_rule]: "((=) ===> rel_expression rel_flip_index (=)) (%x. x) index_flip_expression"
+    unfolding rel_fun_def by auto
+
+  have rel_flip_index_index_flip_var_raw: "rel_flip_index v (index_flip_var_raw v)" for v
+    by (simp add: rel_flip_index_def)
+  have rel_set_rel_flip_index_index_flip_var_raw: "rel_set rel_flip_index vs (index_flip_var_raw ` vs)" for vs
+    by (subst rel_set_rel_flip_index, rule)
+  have Fx: "F x = (F \<circ> index_flip_mem2) y" if "rel_mem2 rel_flip_index x y" for F::"mem2\<Rightarrow>'c" and x y
+    using that apply transfer apply (auto simp: rel_flip_index_def[abs_def])
+    by (metis (full_types) rel_fun_def)
+  then have inv_embedding_index_flip_mem2: "(rel_mem2 rel_flip_index ===> (=)) (inv embedding \<circ> f) (inv embedding \<circ> (f \<circ> index_flip_mem2))" for f
+    apply (rule_tac rel_funI) by simp
+
+  have "rel_substitute1x rel_flip_index rel_flip_index s (index_flip_substitute1 s)" for s
+    unfolding rel_substitute1x_def  
+    using Fx
+    by (metis (mono_tags, lifting) index_flip_var_raw_substitution1_footprint rel_flip_index_def rel_funI rel_set_rel_flip_index substitution1_function_index_flip substitution1_variable_index_flip)
+  
+  then have index_flip_substitute1_transfer [transfer_rule]:
+    "((=) ===> subR) (%x. x) index_flip_substitute1"
+    unfolding subR_def rel_fun_def by auto
+  have "index_flip_expression e = f" if that[transfer_rule]: "rel_expression rel_flip_index (=) e f" for e f :: "'c expression"
+    apply transfer by rule
+  then have [transfer_rule]: "(rel_expression rel_flip_index (=) ===> rel_expression (=) (=)) index_flip_expression id"
+    apply (rule_tac rel_funI) by (simp add: rel_expression_eq)
+
+  have [transfer_rule]: "(list_all2 subR ===> rel_expression rel_flip_index (=) ===> rel_expression rel_flip_index (=))
+   subst_expression subst_expression"
+    unfolding subR_def
+    by transfer_prover
+
+  have "(rel_expression (=) (=))
+        (index_flip_expression (subst_expression \<sigma> e))
+        (id (subst_expression (map index_flip_substitute1 \<sigma>) (index_flip_expression e)))"
+    apply transfer_prover_start
+           apply transfer_step+
+    by simp
+  then
+  show "index_flip_expression (subst_expression \<sigma> e) = subst_expression (map index_flip_substitute1 \<sigma>) (index_flip_expression e)"
+    unfolding rel_expression_eq id_def by assumption
+qed
 
 
 section \<open>ML code\<close>
